SStructTT/SStruct/Runtime/Progress.lean
@@ -46,11 +46,11 @@ lemma Resolved.progressX {H : Heap Srt} {a b c A} :
         cases m1
         all_goals simp_all[Cell.tm]; cases rsm
         case lam m1 _ _ _ =>
-        have ⟨Hx, lk, _⟩ := lk.merge mrg
-        existsi Hx, m1.[.null/]
-        constructor
-        constructor
-        assumption
+          have ⟨Hx, lk, _⟩ := lk.merge mrg
+          existsi Hx, m1.[.null/]
+          constructor
+          constructor
+          assumption
     case ptr => right; aesop
   case app_ex mrg erm ern ihm ihn =>
     subst_vars; cases mrg; cases rs
@@ -59,14 +59,14 @@ lemma Resolved.progressX {H : Heap Srt} {a b c A} :
       match ihm rfl rfl rsm ps1 with
       | .inl ⟨H, m1, st⟩ =>
         have ⟨Hx, x, st⟩ := st.merge mrg
-        exists Hx, .app x n
+        existsi Hx, .app x n
         constructor; assumption
       | .inr ⟨l1, e⟩ =>
         subst_vars
         match ihn rfl rfl rsn ps2 with
         | .inl ⟨H, n1, st⟩ =>
           have ⟨Hx, x, st⟩ := st.merge mrg.sym
-          exists Hx, .app (.ptr l1) x
+          existsi Hx, .app (.ptr l1) x
           constructor; assumption
         | .inr ⟨l2, e⟩ =>
           clear ihm ihn; subst_vars
@@ -76,11 +76,139 @@ lemma Resolved.progressX {H : Heap Srt} {a b c A} :
           cases m1
           all_goals simp_all[Cell.tm]; cases rsm
           case lam m1 _ _ _ =>
-          have ⟨Hx, lk, _⟩ := lk.merge mrg
-          existsi Hx, m1.[.ptr l2/]
-          constructor
-          constructor
-          assumption
+            have ⟨Hx, lk, _⟩ := lk.merge mrg
+            existsi Hx, m1.[.ptr l2/]
+            constructor
+            constructor
+            assumption
+    case ptr => right; aesop
+  case tup_im s _ _ _ erm ihm =>
+    subst_vars; cases rs
+    case tup mrg rsm rsn =>
+      have ⟨_, e⟩ := rsn.null_inv; subst e
+      cases ps
+      case tup_M h ps1 ps2 =>
+        match ihm rfl rfl rsm ps1 with
+        | .inl ⟨H, m1, st⟩ =>
+          have ⟨Hx, x, st⟩ := st.merge mrg
+          left; existsi Hx, .tup x .null s
+          constructor; assumption
+        | .inr ⟨l1, e⟩ =>
+          exfalso; apply h; assumption
+      case tup_N h _ =>
+        exfalso; apply h .null
+    case ptr => right; aesop
+  case tup_ex s _ mrg _ _ _ ihm ihn =>
+    subst_vars; cases mrg; cases rs
+    case tup m n mrg rsm rsn =>
+      cases ps
+      case tup_M h ps1 ps2 =>
+        match ihm rfl rfl rsm ps1 with
+        | .inl ⟨H, m1, st⟩ =>
+          have ⟨Hx, x, st⟩ := st.merge mrg
+          left; existsi Hx, .tup x n s
+          constructor; assumption
+        | .inr ⟨l1, e⟩ =>
+          exfalso; apply h; assumption
+      case tup_N ps1 h ps2 =>
+        match ihn rfl rfl rsn ps2 with
+        | .inl ⟨H, m1, st⟩ =>
+          have ⟨Hx, x, st⟩ := st.merge mrg.sym
+          left; existsi Hx, .tup m x s
+          constructor; assumption
+        | .inr ⟨l1, e⟩ =>
+          exfalso; apply h; subst e; constructor
+    case ptr => right; aesop
+  case prj_im mrg _ erm _ ihm _ =>
+    subst_vars; cases mrg; cases rs
+    case prj rsm rsn =>
+      left; cases ps; case prj m n mrg ps =>
+      match ihm rfl rfl rsm ps with
+      | .inl ⟨H, m1, st⟩ =>
+        have ⟨Hx, x, st⟩ := st.merge mrg
+        existsi Hx, .prj x n
+        constructor; assumption
+      | .inr ⟨l, e⟩ =>
+        subst_vars
+        have vl := rsm.ptr_value
+        have ⟨m1, m2, e⟩ := erm.sig_canonical Conv.R vl; subst e
+        cases rsm; case ptr H m0 lk rsm =>
+        cases m0
+        all_goals simp_all[Cell.tm]; cases rsm
+        case box.tup l _ _ _ rsm rsn =>
+          have ⟨Hx, lk, mrg⟩ := lk.merge mrg
+          existsi Hx, n.[.null,.ptr l/]
+          constructor; assumption
+        case tup.tup rsm rsn =>
+          have ⟨_, _, _, _, erm⟩ := erm.tup_preimage
+          have ⟨_, _, _, _⟩ := erm.toStatic.tup_inv; subst_vars
+          have ⟨_, _, _, _⟩ := erm.tup_im_inv; subst_vars
+          exfalso; have ⟨_, e⟩ := rsn.null_inv; cases e
+    case ptr => right; aesop
+  case prj_ex mrg _ erm _ ihm _ =>
+    subst_vars; cases mrg; cases rs
+    case prj rsm rsn =>
+      left; cases ps; case prj m n mrg ps =>
+      match ihm rfl rfl rsm ps with
+      | .inl ⟨H, m1, st⟩ =>
+        have ⟨Hx, x, st⟩ := st.merge mrg
+        existsi Hx, .prj x n
+        constructor; assumption
+      | .inr ⟨l, e⟩ =>
+        subst_vars
+        have vl := rsm.ptr_value
+        have ⟨m1, m2, e⟩ := erm.sig_canonical Conv.R vl; subst e
+        cases rsm; case ptr H m0 lk rsm =>
+        cases m0
+        all_goals simp_all[Cell.tm]; cases rsm
+        case tup.tup l1 l2 _ _ _ rsm rsn =>
+          have ⟨Hx, lk, mrg⟩ := lk.merge mrg
+          existsi Hx, n.[.ptr l2,.ptr l1/]
+          constructor; assumption
+        case box.tup rsm rsn =>
+          have ⟨_, _, _, _, erm⟩ := erm.tup_preimage
+          have ⟨_, _, _, _⟩ := erm.toStatic.tup_inv; subst_vars
+          have ⟨_, _, _, _, er, _⟩ := erm.tup_ex_inv
+          cases rsn; exfalso; apply er.null_preimage
+    case ptr => right; aesop
+  case tt =>
+    subst_vars; cases rs
+    case tt => cases ps
+    case ptr => right; aesop
+  case ff =>
+    subst_vars; cases rs
+    case ff => cases ps
+    case ptr => right; aesop
+  case ite mrg _ erm _ _ ihm ihn1 ihn2 =>
+    subst_vars; cases mrg; cases rs
+    case ite mrg rsm rsn1 rsn2 =>
+      left; cases ps; case ite m n1 n2 ps =>
+      match ihm rfl rfl rsm ps with
+      | .inl ⟨H, m1, st⟩ =>
+        have ⟨Hx, x, st⟩ := st.merge mrg
+        existsi Hx, .ite x n1 n2
+        constructor; assumption
+      | .inr ⟨l, e⟩ =>
+        subst_vars
+        have vl := rsm.ptr_value
+        cases erm.bool_canonical Conv.R vl with
+        | inl e =>
+          subst e
+          cases rsm; case ptr m0 lk rsm =>
+          cases m0
+          all_goals simp_all[Cell.tm]; cases rsm
+          case tt =>
+            have ⟨Hx, lk, _⟩ := lk.merge mrg
+            existsi Hx, n1
+            constructor; assumption
+        | inr e =>
+          cases rsm; case ptr m0 lk rsm =>
+          cases m0
+          all_goals simp_all[Cell.tm]; cases rsm
+          case ff =>
+            have ⟨Hx, lk, _⟩ := lk.merge mrg
+            existsi Hx, n2
+            constructor; assumption
     case ptr => right; aesop
   case drop ihm ihn =>
     subst_vars; clear ihm ihn
@@ -89,7 +217,6 @@ lemma Resolved.progressX {H : Heap Srt} {a b c A} :
     case ptr => right; aesop
   case rw => subst_vars; aesop
   case conv => subst_vars; aesop
-  all_goals sorry
 
 lemma Resolved.progress {H : Heap Srt} {a b c A} :
     [] ;; [] ;; H ⊢ a ▷ b ◁ c : A ->
